Some definitions were modified, mainly the definition of substitution, since it had some problems.

Lambda/Defs.lean
@@ -47,15 +47,9 @@ notation:70 "↓" => Lambda.unshift
 @[simp]
 def subst (v : Lambda) (n : Nat) (e : Lambda) :=
   match v with
-  | var m =>
-    if m < n then
-      var m
-    else if n = m then
-      (↑) 0 n e
-    else
-      var (m - 1)
+  | var m => if n = m then e else m
   | app v₁ v₂ => app (v₁.subst n e) (v₂.subst n e)
-  | abs v₁ => abs $ v₁.subst (n + 1) e
+  | abs v₁ => abs $ v₁.subst (n + 1) ((↑) 0 1 e)
 
 notation t " [" k " := " s "]" => Lambda.subst t k s
 
