Lambda/Confluence.lean
@@ -17,41 +17,25 @@ lemma abs_reduction {N N' : Lambda} : λ N →βp λ N' ↔ N →βp N' := by
     . apply BetaP.abs
 
 @[simp]
-lemma app_beta (N₁ N₂ N' : Lambda) : (N₁.app N₂).beta N' = (N₁.beta N').app (N₂.beta N') := by
+lemma app_beta {N₁ N₂ N' : Lambda} : (N₁.app N₂).beta N' = (N₁.beta N').app (N₂.beta N') := by
     conv => lhs; unfold beta; simp; rw [← beta, ← beta]
 
-lemma shift_beta {i j : Nat} {N N' : Lambda} :
-    ((↑) (i + 1) j N).beta ((↑) i j N') = (↑) i j (N.beta N') := by
-    induction N generalizing i j with
-    | var k =>
-        sorry
-    | app N₁ N₂ ih1 ih2 =>
-        simp; constructor <;> first | apply ih1 | apply ih2
-    | abs N ih =>
-        simp
-        sorry
+lemma betap_appl {N₁ N₂ N' : Lambda} : N₁ →βp N₂ → N₁.app N' →βp N₂.app N' := by
+    intros; apply BetaP.app; assumption; rfl
 
-lemma subst_shift (i j : Nat) (N N' : Lambda) : N →βp N' → (↑) i j N →βp (↑) i j N' := by
-    intro NreN'
-    induction NreN' generalizing i j with
-    | refl => rfl
-    | abs _ _ _ ih =>
-        simp; apply ih
-    | app _ _ _ _ _ _ ih1 ih2 =>
-        simp; apply BetaP.app <;> (first | apply ih1 | apply ih2)
-    | subst M₁ M₂ N₁ N₂ Mre Nre ih1 ih2 =>
-        simp
-        conv => rhs; apply Eq.symm shift_beta
-        apply BetaP.subst <;> first | apply ih1 | apply ih2
+lemma betap_appr {N₁ N₂ N' : Lambda} : N₁ →βp N₂ → N'.app N₁ →βp N'.app N₂ := by
+    intros; apply BetaP.app; rfl; assumption
 
-lemma subst_reduction (M N N' : Lambda) (n : Nat) : N →βp N' → M[n := N] →βp M[n := N'] := by
-    intros
-    induction M generalizing n with
-    | var k =>
-        simp; split_ifs; simp
-        apply subst_shift; assumption; rfl
-    | app M₁ M₂ ih1 ih2 =>
+lemma shift_conservation {i j : Nat} {N N' : Lambda} : N →βp N' → (↑) i j N →βp (↑) i j N' := by
+    intro h
+    induction h generalizing i j with
+    | refl _ => rfl
+    | abs N₁ N₂ h ih => simp; apply ih
+    | app M₁ M₂ N₁ N₂ hm hn ihm ihn =>
         simp
-        apply BetaP.app <;> repeat first | apply ih1 | apply ih2 | assumption
-    | abs M ih =>
-        simp; apply ih
+        apply BetaP.app
+        apply ihm
+        apply ihn
+    | subst M₁ M₂ N₁ N₂ hm hn ihm ihn =>
+        simp
+        sorry
