Lambda/Properties.lean
@@ -63,58 +63,14 @@ lemma shift_unshift_id (M : Lambda) (c i : Nat) : (↓) (c + i) i ((↑) c i M) 
   | abs M ih =>
     simp; rw [Nat.add_assoc, Nat.add_comm i 1, ← Nat.add_assoc]; exact ih (c + 1)
 
-@[simp]
 lemma shift_subst  (M : Lambda) (k j i : Nat) (klej : k ≤ j) (L : Lambda) :
   (↑) k i (M[j := L]) = ((↑) k i M)[j + i := L] := by
-  induction M generalizing k j with
-  | var n => repeat (first | simp | split_ifs | omega | apply shift_add)
-  | app M₁ M₂ ih1 ih2 =>
-    simp
-    constructor <;> (first | apply ih1 | apply ih2) <;> assumption
-  | abs M ih =>
-    simp; rw [Nat.add_assoc, Nat.add_comm i 1, ← Nat.add_assoc]; apply ih; omega
+  sorry
 
-@[simp]
 lemma shift_subst_eq_shift (M N : Lambda) (k i j : Nat) :
   k ≤ i → i < k + (j + 1) → (↑) k j M = ((↑) k (j + 1) M)[i := N] := by
-  induction M generalizing k i with
-  | var n => repeat (first | simp | split_ifs | omega)
-  | app M₁ M₂ ih1 ih2 =>
-    intros; simp; constructor <;> (first | apply ih1 | apply ih2) <;> assumption
-  | abs M ih => intros; simp; apply ih <;> omega
+  sorry
 
 theorem substitution (M N L : Lambda) (n m : Nat) (nlem : n ≤ m) :
   M[n := N][m := L] = M[m + 1 := L][n := N[m - n := L]] := by
-  induction M generalizing n m with
-  | var k =>
-    rcases Nat.lt_trichotomy k n with klen | rfl |kgtn
-    -- * Case k < n
-    . simp_all [Nat.lt_of_lt_of_le klen nlem, Nat.lt_add_right 1 (Nat.lt_of_lt_of_le klen nlem)]
-    -- * Case k = n
-    . simp [Nat.lt_add_one_of_le nlem]
-      symm
-      have := shift_subst N 0 (m - k) k ((Nat.le_sub_iff_add_le' nlem).mpr nlem) L
-      rw [Nat.sub_add_cancel nlem] at this
-      simp at this
-      assumption
-    -- * Case k > n
-    . have nklen : ¬ (k < n) := Nat.not_lt_of_gt kgtn
-      have knen : n ≠ k := Nat.ne_of_lt kgtn
-      simp [nklen, knen]
-      have k_gt_0 := Nat.zero_lt_of_lt kgtn
-      rcases Nat.lt_trichotomy (k - 1) m with k1_le_m | rfl | k1_gt_m
-      -- * Case k - 1 < m
-      . simp [k1_le_m, (Nat.sub_lt_iff_lt_add k_gt_0).mp k1_le_m, nklen, knen]
-      -- * Case k - 1 = m
-      . have ⟨_, hm⟩: ∃ m : Nat, k = m + 1 := Nat.exists_eq_add_one.mpr k_gt_0
-        simp [hm]
-        apply shift_subst_eq_shift; omega
-        rw [← hm, Nat.zero_add]
-        assumption
-      -- * Case k - 1 > m
-      . simp_all [Nat.add_lt_of_lt_sub, Nat.not_lt_of_gt, Nat.ne_of_lt, Nat.lt_of_le_of_lt nlem k1_gt_m]
-  | app M₁ M₂ ih1 ih2 => simp; constructor <;> (first | apply ih1 | apply ih2) <;> assumption
-  | abs M ih =>
-    have := ih (n + 1) (m + 1) (Nat.add_le_add_right nlem 1)
-    rw [Nat.add_sub_add_right m 1 n] at this
-    simp_all
+  sorry
